Revert "Checkpoint experiment with switching over to Z over nat in more places"
This reverts commit 3c857223fabc2e1be4d43f11cb7df4e0811c59d1.

src/goose_lang/ffi/disk_ffi/impl.v
@@ -26,11 +26,15 @@ Proof.
   refine (mkExtOp DiskOp _ _ () _ _).
 Defined.
 
-Definition block_bytes: Z := 4096.
+Definition block_bytes: nat := Z.to_nat 4096.
 Definition BlockSize {ext: ffi_syntax}: val := #4096.
-Definition Block := vec byte (Z.to_nat block_bytes).
+Definition Block := vec byte block_bytes.
 (* TODO: could use vreplicate; not sure how much easier it is to work with *)
-Definition block0 : Block := list_to_vec (replicate (Z.to_nat block_bytes) (W8 0)).
+Definition block0 : Block := list_to_vec (replicate (Z.to_nat 4096) (W8 0)).
+
+
+Lemma block_bytes_eq : block_bytes = Z.to_nat 4096.
+Proof. reflexivity. Qed.
 
 Global Instance Block0: Inhabited Block := _.
 Global Instance Block_countable : Countable Block := _.
@@ -52,7 +56,7 @@ Definition Block_to_vals {ext: ffi_syntax} (bl:Block) : list val :=
   b2val <$> vec_to_list bl.
 
 Lemma length_Block_to_vals {ext: ffi_syntax} b :
-    Z.of_nat $ length (Block_to_vals b) = block_bytes.
+    length (Block_to_vals b) = block_bytes.
 Proof.
   rewrite /Block_to_vals length_fmap length_vec_to_list //.
 Qed.
